Added init and phase1 invariants to paxos, and lemmas maintaining them

ironfleet/src/Dafny/Distributed/Protocol/RSL/PerformanceProof/PerformanceProof.i.dfy
@@ -13,17 +13,17 @@ module RslPerformanceProof_i {
 import opened TimestampedRslPerformanceProof_i
 import opened CommonProof__Constants_i
 
-predicate RslAssumption(s:TimestampedRslState)
+predicate {:verify false} RslAssumption(s:TimestampedRslState)
 {
   |s.t_replicas| > 0
 }
 
-predicate RslConsistency(s:TimestampedRslState)
+predicate {:verify false} RslConsistency(s:TimestampedRslState)
 {
   ConstantsAllConsistentInv(UntimestampRslState(s))
 }
 
-predicate ViewAlwaysZero(s:TimestampedRslState)
+predicate {:verify false} ViewAlwaysZero(s:TimestampedRslState)
 {
   && (forall idx:: 0 <= idx < |s.t_replicas|
     ==>
@@ -31,17 +31,22 @@ predicate ViewAlwaysZero(s:TimestampedRslState)
     )
 }
 
-predicate AlwaysInvariant(s:TimestampedRslState)
+predicate {:verify false} AlwaysInvariant(s:TimestampedRslState)
 {
   && ViewAlwaysZero(s)
 }
 
-predicate InitInvariant(s:TimestampedRslState)
+predicate {:verify false} InitInvariant(s:TimestampedRslState)
   requires RslConsistency(s)
 {
-  && (forall idx:: 0 <= idx < |s.t_replicas|
-    ==> 
-    TimeEq(s.t_replicas[idx].ts, TimeZero())
+  && (0 < |s.t_replicas|
+    ==>
+    var r := s.t_replicas[0].v.replica.proposer;
+    if s.t_replicas[0].v.nextActionIndex == 0 then
+      TimeEq(s.t_replicas[0].ts, TimeZero())
+    else
+      && s.t_replicas[0].v.nextActionIndex == 1
+      && TimeLe(s.t_replicas[0].ts, Timeout() + L)
     )
 
   && (0 < |s.t_replicas| ==>
@@ -49,20 +54,94 @@ predicate InitInvariant(s:TimestampedRslState)
     && p.current_state == 0
     && BalLt(p.max_ballot_i_sent_1a, p.election_state.current_view)
   )
+
+  && (forall idx :: 0 <= idx < |s.t_replicas|
+  ==> s.t_replicas[idx].v.replica.acceptor.max_bal == Ballot(0, 0)
+  && s.t_replicas[idx].v.replica.proposer.current_state == 0
+  && s.t_replicas[idx].v.replica.executor.next_op_to_execute == OutstandingOpUnknown()
+  && s.t_replicas[idx].v.replica.learner.unexecuted_learner_state == map[]
+  )
+
+  && (forall pkt :: pkt in s.t_environment.sentPackets
+  ==> pkt.msg.v.RslMessage_Heartbeat?
+  )
 }
 
-predicate Phase1Invariant(s:TimestampedRslState)
+predicate {:verify false} Phase1aInvariant(s:TimestampedRslState)
   requires RslConsistency(s)
 {
+  && (forall idx :: 0 <= idx < |s.t_replicas|
+    ==>
+  && s.t_replicas[idx].v.replica.executor.next_op_to_execute == OutstandingOpUnknown()
+  && s.t_replicas[idx].v.replica.learner.unexecuted_learner_state == map[]
+  )
+
   && (0 < |s.t_replicas| ==>
-    && TimeEq(s.t_replicas[0].ts, L)
+    && TimeLe(s.t_replicas[0].ts, TimeBound1aSent())
   )
   && (0 < |s.t_replicas| ==>
     && s.t_replicas[0].v.replica.proposer.current_state == 1
   )
+
+  && (forall pkt :: pkt in s.t_environment.sentPackets
+  ==>
+   || pkt.msg.v.RslMessage_Heartbeat?
+   || pkt.msg.v.RslMessage_1a?
+  )
+
+  && (forall pkt :: pkt in s.t_environment.sentPackets
+      && pkt.msg.v.RslMessage_1a?
+  ==> TimeLe(pkt.msg.ts, TimeBound1aSent())
+  )
+
+  && (forall idx :: 0 < idx < |s.t_replicas|
+  ==>
+  if s.t_replicas[idx].v.replica.acceptor.max_bal == Ballot(0, 0) then
+    // TODO: s.t_replicas[idx].ts == TimeZero() 
+    true
+  else
+    (&& s.t_replicas[idx].v.replica.acceptor.max_bal == s.t_replicas[0].v.replica.proposer.max_ballot_i_sent_1a
+    && s.t_replicas[idx].ts == TimeBound1aReceived())
+  )
 }
 
-lemma Init(s:TimestampedRslState, s':TimestampedRslState)
+lemma {:verify false} NextProcessPacket_0_InitGoesToInit(s:TimestampedRslState, s':TimestampedRslState)
+  requires RslAssumption(s);
+  requires ViewAlwaysZero(s)
+  requires RslConsistency(s);
+  requires RslConsistency(s');
+
+  requires s.t_environment.nextStep.LEnvStepHostIos?;
+  requires s.t_environment.nextStep.actor == s.constants.config.replica_ids[0];
+  requires s.t_environment.nextStep.nodeStep == RslStep(0);
+
+  requires TimestampedRslNextOneReplica(s, s', 0, s.t_environment.nextStep.ios);
+
+  requires InitInvariant(s)
+  ensures InitInvariant(s')
+{
+}
+
+lemma {:verify false} NextProcessPacket_j_InitGoesToInit(s:TimestampedRslState, s':TimestampedRslState, j:int)
+  requires RslAssumption(s);
+  requires ViewAlwaysZero(s)
+  requires RslConsistency(s);
+  requires RslConsistency(s');
+  requires 0 <= j < |s.constants.config.replica_ids|
+
+  requires j > 0;
+
+  requires s.t_environment.nextStep.LEnvStepHostIos?;
+  requires s.t_environment.nextStep.actor == s.constants.config.replica_ids[j];
+
+  requires TimestampedRslNextOneReplica(s, s', j, s.t_environment.nextStep.ios);
+
+  requires InitInvariant(s)
+  ensures InitInvariant(s')
+{
+}
+
+lemma MaybeEnterNewView_1_InitGoesToPhase1a(s:TimestampedRslState, s':TimestampedRslState)
   requires RslAssumption(s);
   requires ViewAlwaysZero(s)
   requires RslConsistency(s);
@@ -75,7 +154,7 @@ lemma Init(s:TimestampedRslState, s':TimestampedRslState)
   requires TimestampedRslNextOneReplica(s, s', 0, s.t_environment.nextStep.ios);
 
   requires InitInvariant(s)
-  ensures Phase1Invariant(s')
+  ensures Phase1aInvariant(s')
 {
 }
 
